Coq/EC/EC_P384_Abstract.v
@@ -53,8 +53,7 @@ Local Arguments reverse [n] [a]%type_scope {Inh_a} _.
 Local Arguments bvSub [n] _ _.
 Local Arguments SAWCorePrelude.map [a]%type_scope {Inh_a} [b]%type_scope f%function_scope _ _.
 
-
-Definition mul_scalar_rwnaf_odd_loop_body_gen (wsize : nat)(s : bitvector 384) :=
+Definition mul_scalar_rwnaf_odd_loop_body_abstract (wsize : nat)(s : bitvector 384) :=
 (drop Bool 368 16
    (bvSub
       (bvURem 384 s
@@ -69,11 +68,11 @@ shiftR 384 bool false
               (shiftL 384 bool false (bvNat 384 1) wsize)))
         (shiftL 384 bool false (bvNat 384 1) wsize))) wsize).
 
-Theorem mul_scalar_rwnaf_odd_loop_body_gen_equiv : forall s,
-  mul_scalar_rwnaf_odd_loop_body_gen 5 s = mul_scalar_rwnaf_odd_loop_body s.
+Theorem mul_scalar_rwnaf_odd_loop_body_abstract_equiv : forall s,
+  mul_scalar_rwnaf_odd_loop_body_abstract 5 s = mul_scalar_rwnaf_odd_loop_body s.
 
   intros.
-  unfold mul_scalar_rwnaf_odd_loop_body, mul_scalar_rwnaf_odd_loop_body_gen.
+  unfold mul_scalar_rwnaf_odd_loop_body, mul_scalar_rwnaf_odd_loop_body_abstract.
   removeCoerce.
   simpl.
   reflexivity.
@@ -90,20 +89,29 @@ Require Import Nat.
 Require Import List.
 Require Import Arith.
 
-Definition mul_scalar_rwnaf_odd_gen wsize numWindows s :=
+(* The abstract form of the double-and-add loop.
+The function uses scanl to build a list of intermediate results and uses
+hd to get the last result from the head of the list. The form of hd used
+requires a default value that is returned when the list is empty (but the 
+proof will show that the list is never empty). To produce this default valuu,
+we use the Inhabited typeclass instances that proves that certain types are
+inhabited, and the inhabitant function that produces a value from an inhabited 
+type.
+*)
+Definition mul_scalar_rwnaf_odd_abstract wsize numWindows s :=
   List.map (fun x : bitvector 16 * bitvector 384 => fst x)
   (scanl
      (fun (__p2 : bitvector 16 * bitvector 384) (_ : Integer) =>
-      mul_scalar_rwnaf_odd_loop_body_gen wsize (snd __p2)) (toN_int numWindows)
-     (mul_scalar_rwnaf_odd_loop_body_gen wsize s)) ++
+      mul_scalar_rwnaf_odd_loop_body_abstract wsize (snd __p2)) (toN_int numWindows)
+     (mul_scalar_rwnaf_odd_loop_body_abstract wsize s)) ++
 [drop Bool 368%nat 16%nat
    (snd
       (hd (inhabitant (Inhabited_prod (bitvector 16) (bitvector 384)))
          (rev
             (scanl
                (fun (__p2 : bitvector 16 * bitvector 384) (_ : Integer) =>
-                mul_scalar_rwnaf_odd_loop_body_gen wsize (snd __p2)) 
-               (toN_int numWindows) (mul_scalar_rwnaf_odd_loop_body_gen wsize s)))))].
+                mul_scalar_rwnaf_odd_loop_body_abstract wsize (snd __p2)) 
+               (toN_int numWindows) (mul_scalar_rwnaf_odd_loop_body_abstract wsize s)))))].
 
 
 Local Open Scope Z_scope.
@@ -129,8 +137,8 @@ Qed.
 
 Require Import Coq.ZArith.Zdigits.
 
-Theorem mul_scalar_rwnaf_odd_gen_equiv : forall s,
-  to_list (mul_scalar_rwnaf_odd s) = (mul_scalar_rwnaf_odd_gen 5 74 s).
+Theorem mul_scalar_rwnaf_odd_abstract_equiv : forall s,
+  to_list (mul_scalar_rwnaf_odd s) = (mul_scalar_rwnaf_odd_abstract 5 74 s).
 
   intros.
   unfold mul_scalar_rwnaf_odd.
@@ -159,38 +167,38 @@ Theorem mul_scalar_rwnaf_odd_gen_equiv : forall s,
     replace (to_list (SAWCoreVectorsAsCoqVectors.scanl t1 t2 n f a v)) with (scanl f (to_list v) a); [idtac | symmetry; apply toList_scanl_equiv]
   end.
 
-  rewrite <- mul_scalar_rwnaf_odd_loop_body_gen_equiv.
+  rewrite <- mul_scalar_rwnaf_odd_loop_body_abstract_equiv.
   rewrite (scanl_ext _ (fun (__p2 : bitvector 16 * bitvector 384) (_ : Integer) =>
-      mul_scalar_rwnaf_odd_loop_body_gen 5 (snd __p2))).
+      mul_scalar_rwnaf_odd_loop_body_abstract 5 (snd __p2))).
 
   rewrite ecFromTo_0_n_equiv.
   reflexivity.
 
   intros.
   symmetry.
-  apply mul_scalar_rwnaf_odd_loop_body_gen_equiv.
+  apply mul_scalar_rwnaf_odd_loop_body_abstract_equiv.
 
   lia.
 
 Qed.
 
-Definition mul_scalar_rwnaf_gen wsize nw s := 
-  mul_scalar_rwnaf_odd_gen wsize nw
+Definition mul_scalar_rwnaf_abstract wsize nw s := 
+  mul_scalar_rwnaf_odd_abstract wsize nw
     (bvOr s (intToBv 384%nat 1)).
 
 Theorem mul_scalar_rwnaf_equiv : forall s,
-  to_list (mul_scalar_rwnaf s) = mul_scalar_rwnaf_gen 5 74 s.
+  to_list (mul_scalar_rwnaf s) = mul_scalar_rwnaf_abstract 5 74 s.
 
   intros.
   unfold mul_scalar_rwnaf.
-  rewrite mul_scalar_rwnaf_odd_gen_equiv.
-  Local Opaque mul_scalar_rwnaf_odd_gen.
+  rewrite mul_scalar_rwnaf_odd_abstract_equiv.
+  Local Opaque mul_scalar_rwnaf_odd_abstract.
   simpl.
   reflexivity.
 
 Qed.
 
-Definition select_point_gen x t :=
+Definition select_point_abstract x t :=
   fold_left
   (fun acc p =>
    select_point_loop_body x acc (fst p) (snd p))
@@ -209,11 +217,11 @@ Theorem to_list_length : forall (A : Type)(n : nat)(x : Vector.t A n),
 Qed.
 
 
-Theorem select_point_gen_equiv : forall x t,
-  select_point x t = select_point_gen x (to_list t).
+Theorem select_point_abstract_equiv : forall x t,
+  select_point x t = select_point_abstract x (to_list t).
 
   intros.
-  unfold select_point, select_point_gen.
+  unfold select_point, select_point_abstract.
   removeCoerce.
   rewrite ecFoldl_foldl_equiv.
   rewrite toList_zip_equiv. 
@@ -336,7 +344,7 @@ Section PointMul.
 
   Definition pre_comp_table := pre_comp_table felem_sqr felem_mul felem_sub felem_add .
 
-  Definition pre_comp_table_gen pred_tsize p :=
+  Definition pre_comp_table_abstract pred_tsize p :=
     scanl
   (fun
      (z : CryptolPrimitivesForSAWCore.seq 3%nat
@@ -348,11 +356,11 @@ Section PointMul.
      (point_double felem_sqr felem_mul felem_sub felem_add p) z)
   (map (BinIntDef.Z.add (BinIntDef.Z.of_nat 1)) (toN_int pred_tsize)) p .
 
-  Theorem pre_comp_table_gen_equiv : forall p,
-    to_list (pre_comp_table p) = pre_comp_table_gen 14%nat p.
+  Theorem pre_comp_table_abstract_equiv : forall p,
+    to_list (pre_comp_table p) = pre_comp_table_abstract 14%nat p.
 
     intros. 
-    unfold pre_comp_table_gen, pre_comp_table, EC_P384_5.pre_comp_table.
+    unfold pre_comp_table_abstract, pre_comp_table, EC_P384_5.pre_comp_table.
     removeCoerce.
     removeCoerce.
     rewrite toList_scanl_equiv.
@@ -370,7 +378,7 @@ Section PointMul.
   Definition conditional_point_opp (t : bitvector 64) (p : point): point :=
     Vector.cons (sawAt _ _ p 0%nat) (Vector.cons (felem_cmovznz t (sawAt _ _ p 1%nat) (field_opp (sawAt _ _ p 1%nat))) (Vector.cons (sawAt _ _ p 2%nat) (Vector.nil _))).
 
-  Definition double_add_body_gen pred_wsize t p id :=
+  Definition double_add_body_abstract pred_wsize t p id :=
     EC_P384_5.point_add felem_sqr felem_mul felem_sub
   felem_add false
   (fold_left
@@ -384,7 +392,7 @@ Section PointMul.
   (conditional_point_opp
      (point_id_to_limb
         (shiftR 16 bool false id 15))
-     (select_point_gen
+     (select_point_abstract
         (sign_extend_16_64
            (bvSShr 15%nat
               (bvAdd 16
@@ -395,8 +403,8 @@ Section PointMul.
                       (bvSShr 15%nat id 15)
 )) 1%nat)) t)).
 
-  Theorem double_add_body_gen_equiv : forall t p id,
-    double_add_body t p id = double_add_body_gen 4 (to_list t) p id.
+  Theorem double_add_body_abstract_equiv : forall t p id,
+    double_add_body t p id = double_add_body_abstract 4 (to_list t) p id.
 
     intros.
     unfold double_add_body, EC_P384_5.double_add_body.
@@ -405,7 +413,7 @@ Section PointMul.
 
     replace (to_list (ecFromTo 0%nat 4%nat Integer PLiteralInteger))
       with (toN_int 4%nat).
-    repeat rewrite select_point_gen_equiv.
+    repeat rewrite select_point_abstract_equiv.
     reflexivity.
 
     symmetry.
@@ -413,24 +421,24 @@ Section PointMul.
 
   Qed.
 
-  Definition point_mul_gen wsize nw pred_tsize p s : point := 
+  Definition point_mul_abstract wsize nw pred_tsize p s : point := 
     EC_P384_5.conditional_subtract_if_even felem_sqr felem_mul
   felem_sub felem_add field_opp
   (fold_left
-     (double_add_body_gen (pred wsize) (pre_comp_table_gen pred_tsize p))
-     (skipn 1 (rev (mul_scalar_rwnaf_gen wsize nw s)))
-     (select_point_gen
+     (double_add_body_abstract (pred wsize) (pre_comp_table_abstract pred_tsize p))
+     (skipn 1 (rev (mul_scalar_rwnaf_abstract wsize nw s)))
+     (select_point_abstract
         (sign_extend_16_64
            (bvSShr 15
-              (nth (S (S nw)) (mul_scalar_rwnaf_gen wsize nw s)
+              (nth (S (S nw)) (mul_scalar_rwnaf_abstract wsize nw s)
                  (bvNat 16%nat 0%nat))
               1%nat) )
-        (pre_comp_table_gen pred_tsize p))) s
-  (nth 0 (pre_comp_table_gen pred_tsize p)
+        (pre_comp_table_abstract pred_tsize p))) s
+  (nth 0 (pre_comp_table_abstract pred_tsize p)
      (inhabitant (ecNumber 0%nat Integer PLiteralInteger))).
 
-  Theorem point_mul_gen_equiv : forall p s,
-    point_mul p s = point_mul_gen 5 74 14 p s.
+  Theorem point_mul_abstract_equiv : forall p s,
+    point_mul p s = point_mul_abstract 5 74 14 p s.
 
     intros.
     unfold point_mul, EC_P384_5.point_mul.
@@ -440,22 +448,22 @@ Section PointMul.
     Local Opaque fold_left.
     simpl.
     rewrite (fold_left_ext _
-      (double_add_body_gen 4%nat
-        (pre_comp_table_gen 14%nat p))
+      (double_add_body_abstract 4%nat
+        (pre_comp_table_abstract 14%nat p))
     ).
     rewrite toList_drop_equiv.
     rewrite toList_reverse_equiv.
     rewrite mul_scalar_rwnaf_equiv.
 
-    rewrite select_point_gen_equiv.
-    rewrite pre_comp_table_gen_equiv.
+    rewrite select_point_abstract_equiv.
+    rewrite pre_comp_table_abstract_equiv.
 
-    unfold point_mul_gen.
+    unfold point_mul_abstract.
     rewrite sawAt_nth_equiv.
     rewrite mul_scalar_rwnaf_equiv.
 
     rewrite sawAt_nth_equiv.
-    rewrite pre_comp_table_gen_equiv.
+    rewrite pre_comp_table_abstract_equiv.
 
     reflexivity.
 
@@ -463,10 +471,10 @@ Section PointMul.
     lia.
 
     intros.
-    rewrite <- pre_comp_table_gen_equiv.
+    rewrite <- pre_comp_table_abstract_equiv.
     unfold pre_comp_table.
   
-    rewrite <- double_add_body_gen_equiv.
+    rewrite <- double_add_body_abstract_equiv.
     reflexivity.
 
   Qed.
